wip

Foundation/Modal/Kripke/AxiomVer.lean
@@ -7,40 +7,36 @@ open Formula.Kripke
 
 namespace Kripke
 
-abbrev FrameClass.isolated : FrameClass := { F | Isolated F }
 
-@[simp]
-lemma FrameClass.isolated.nonempty : FrameClass.isolated.Nonempty := by
-  use ⟨Unit, λ _ _ => False⟩;
-  tauto;
+lemma validate_AxiomVer_of_isolated {F : Frame} (h : Isolated F) : F ⊧ (Axioms.Ver (.atom 0)) := by
+  intro V x y Rxy;
+  have := h Rxy;
+  contradiction;
 
-instance FrameClass.isolated.definability : FrameClass.isolated.DefinedByFormula (Axioms.Ver (.atom 0)) := ⟨by
-  intro F;
-  simp only [Set.mem_setOf_eq, Set.mem_singleton_iff, ValidOnFrame.models_iff, forall_eq];
-  constructor;
-  . intro h V x y Rxy;
-    have := h Rxy;
-    contradiction;
-  . intro h x y Rxy;
-    have := h (λ _ _ => False) x y Rxy;
-    simp [Formula.Kripke.Satisfies] at this;
-⟩
+lemma isolated_of_validate_AxiomVer {F : Frame} (h : F ⊧ (Axioms.Ver (.atom 0))) : Isolated F := by
+  intro x y Rxy;
+  have := h (λ _ _ => False) x y Rxy;
+  simp [Formula.Kripke.Satisfies] at this;
 
-end Kripke
 
-namespace Kripke
-
+section canonicality
 
 open Entailment
 
 variable {S} [Entailment (Formula ℕ) S]
-variable {𝓢 : S} [Entailment.Consistent 𝓢]
+variable {𝓢 : S} [Entailment.Consistent 𝓢] [Entailment.K 𝓢]
 
-instance [Entailment.Ver 𝓢] : Canonical 𝓢 FrameClass.isolated := ⟨by
+open Formula.Kripke
+open Entailment
+open MaximalConsistentTableau
+open canonicalModel
+
+protected lemma Canonical.isolated [Entailment.HasAxiomVer 𝓢] : Isolated (canonicalFrame 𝓢).Rel := by
   intro x y Rxy;
   have : (canonicalModel 𝓢) ⊧ □⊥ := iff_valid_on_canonicalModel_deducible.mpr axiomVer!
   exact this x _ Rxy;
-⟩
+
+end canonicality
 
 end Kripke
 
