Foundation/Modal/Kripke/Hilbert/KT4B.lean
@@ -4,36 +4,59 @@ import Foundation.Modal.Kripke.Filteration
 namespace LO.Modal
 
 open Kripke
+open Hilbert.Kripke
 open Geachean
 
 abbrev Kripke.FrameClass.symm_preorder : FrameClass := { F | Reflexive F ∧ Transitive F ∧ Symmetric F }
-abbrev Kripke.FiniteFrameClass.symm_preorder : FiniteFrameClass := { F | Reflexive F.Rel ∧ Transitive F.Rel ∧ Symmetric F.Rel }
+abbrev Kripke.FrameClass.finite_symm_preorder: FrameClass := { F | F.IsFinite ∧ Reflexive F.Rel ∧ Transitive F.Rel ∧ Symmetric F.Rel }
+
+namespace Kripke.FrameClass.symm_preorder
+
+lemma isMultiGeachean : FrameClass.symm_preorder = FrameClass.multiGeachean {⟨0, 0, 1, 0⟩, ⟨0, 2, 1, 0⟩, ⟨0, 1, 0, 1⟩} := by
+  ext F;
+  simp [Geachean.reflexive_def, Geachean.transitive_def, Geachean.symmetric_def, MultiGeachean]
+
+@[simp]
+lemma nonempty : FrameClass.symm_preorder.Nonempty := by simp [isMultiGeachean]
+
+lemma validates_HilbertKT4B : Kripke.FrameClass.symm_preorder.Validates Hilbert.KT4B.axioms := by
+  apply FrameClass.Validates.withAxiomK;
+  rintro F ⟨_, _, _⟩ _ (rfl | rfl | rfl);
+  . exact validate_AxiomT_of_reflexive $ by assumption;
+  . exact validate_AxiomFour_of_transitive $ by assumption;
+  . exact validate_AxiomB_of_symmetric $ by assumption;
+
+end Kripke.FrameClass.symm_preorder
+
 
 namespace Hilbert.KT4B.Kripke
 
-instance consistent : Entailment.Consistent (Hilbert.KT4B) := by
-  convert Hilbert.Geach.Kripke.consistent (G := {⟨0, 0, 1, 0⟩, ⟨0, 2, 1, 0⟩, ⟨0, 1, 0, 1⟩});
-  exact eq_Geach;
+instance sound : Sound (Hilbert.KT4B) Kripke.FrameClass.symm_preorder :=
+  instSound_of_validates_axioms Kripke.FrameClass.symm_preorder.validates_HilbertKT4B
+
+instance consistent : Entailment.Consistent (Hilbert.KT4B) :=
+  consistent_of_sound_frameclass Kripke.FrameClass.symm_preorder (by simp)
 
 instance canonical : Canonical (Hilbert.KT4B) Kripke.FrameClass.symm_preorder := ⟨⟨Canonical.reflexive, Canonical.transitive, Canonical.symmetric⟩⟩
 
 instance complete : Complete (Hilbert.KT4B) Kripke.FrameClass.symm_preorder := inferInstance
 
 open finestFilterationTransitiveClosureModel in
-instance finite_complete : Complete (Hilbert.KT4B) Kripke.FiniteFrameClass.symm_preorder := ⟨by
+instance finite_complete : Complete (Hilbert.KT4B) Kripke.FrameClass.finite_symm_preorder := ⟨by
   intro φ hp;
   apply Kripke.complete.complete;
   intro F ⟨F_refl, F_trans, F_symm⟩ V x;
   let M : Kripke.Model := ⟨F, V⟩;
   let FM := finestFilterationTransitiveClosureModel M φ.subformulas;
   apply filteration FM (finestFilterationTransitiveClosureModel.filterOf F_trans) (by aesop) |>.mpr;
-  apply validOnModel_of_validOnFiniteFrameClass hp;
-  . refine ⟨?_, ?_, ?_⟩;
-    . exact reflexive_of_transitive_reflexive (by apply F_trans) F_refl;
-    . exact transitive;
-    . exact symmetric_of_symmetric F_symm;
-  . apply FilterEqvQuotient.finite;
+  apply hp;
+  refine ⟨?_, ?_, ?_, ?_⟩;
+  . apply Frame.isFinite_iff _ |>.mpr
+    apply FilterEqvQuotient.finite;
     simp;
+  . exact reflexive_of_transitive_reflexive (by apply F_trans) F_refl;
+  . exact finestFilterationTransitiveClosureModel.transitive;
+  . exact symmetric_of_symmetric F_symm;
 ⟩
 
 end Hilbert.KT4B.Kripke
