Foundation/Modal/Kripke/Hilbert/KTc.lean
@@ -3,25 +3,43 @@ import Foundation.Modal.Kripke.Hilbert.Geach
 namespace LO.Modal
 
 open Kripke
+open Hilbert.Kripke
 open Geachean
 
-abbrev Kripke.FrameClass.corefl : FrameClass := { F | Coreflexive F }
+namespace Kripke.FrameClass
+
+protected abbrev corefl : FrameClass := { F | Coreflexive F }
+
+namespace corefl
+
+lemma isMultiGeachean : FrameClass.corefl = FrameClass.multiGeachean {⟨0, 1, 0, 0⟩} := by
+  ext F;
+  simp [Geachean.coreflexive_def, MultiGeachean]
+
+@[simp]
+lemma nonempty : FrameClass.corefl.Nonempty := by simp [corefl.isMultiGeachean]
+
+lemma validates_AxiomTc : FrameClass.corefl.ValidatesFormula (Axioms.Tc (.atom 0)) := by
+  rintro F F_corefl _ rfl;
+  apply validate_AxiomTc_of_coreflexive F_corefl;
+
+lemma validates_HilbertKTc : FrameClass.corefl.Validates Hilbert.KTc.axioms := Validates.withAxiomK validates_AxiomTc
+
+end corefl
+
+end Kripke.FrameClass
 
 namespace Hilbert.KTc
 
-instance Kripke.sound : Sound (Hilbert.KTc) Kripke.FrameClass.corefl := by
-  convert Hilbert.Geach.Kripke.sound (G := {⟨0, 1, 0, 0⟩});
-  exact eq_Geach;
-  . unfold Kripke.FrameClass.corefl FrameClass.multiGeachean MultiGeachean;
-    simp [Geachean.reflexive_def, Geachean.coreflexive_def];
+instance Kripke.sound : Sound (Hilbert.KTc) Kripke.FrameClass.corefl :=
+  instSound_of_validates_axioms Kripke.FrameClass.corefl.validates_HilbertKTc
 
-instance Kripke.consistent : Entailment.Consistent (Hilbert.KTc) := by
-  convert Hilbert.Geach.Kripke.consistent (G := {⟨0, 1, 0, 0⟩});
-  exact eq_Geach;
+instance Kripke.consistent : Entailment.Consistent (Hilbert.KTc) :=
+  consistent_of_sound_frameclass Kripke.FrameClass.corefl (by simp)
 
-instance Kripke.canonical : Canonical (Hilbert.KTc) Kripke.FrameClass.corefl := ⟨Canonical.coreflexive⟩
+instance Kripke.canonical : Canonical (Hilbert.KTc) FrameClass.corefl := ⟨Canonical.coreflexive⟩
 
-instance Kripke.complete : Complete (Hilbert.KTc) Kripke.FrameClass.corefl := inferInstance
+instance Kripke.complete : Complete (Hilbert.KTc) FrameClass.corefl := inferInstance
 
 end Hilbert.KTc
 
