Foundation/Modal/Kripke/Hilbert/S5.lean
@@ -4,15 +4,34 @@ import Foundation.Modal.Kripke.Hilbert.KT4B
 namespace LO.Modal
 
 open Kripke
+open Hilbert.Kripke
 open Geachean
 
 namespace Kripke
 
 protected abbrev FrameClass.refl_eucl : FrameClass := { F | Reflexive F ∧ Euclidean F }
 
+namespace FrameClass.refl_eucl
+
+lemma isMultiGeachean : FrameClass.refl_eucl = FrameClass.multiGeachean {⟨0, 0, 1, 0⟩, ⟨1, 1, 0, 1⟩} := by
+  ext F;
+  simp [Geachean.reflexive_def, Geachean.euclidean_def, MultiGeachean]
+
+@[simp]
+lemma nonempty : FrameClass.refl_eucl.Nonempty := by simp [isMultiGeachean]
+
+lemma validates_HilbertS5 : Kripke.FrameClass.refl_eucl.Validates Hilbert.S5.axioms := by
+  apply FrameClass.Validates.withAxiomK;
+  rintro F ⟨_, _⟩ _ (rfl | rfl);
+  . exact validate_AxiomT_of_reflexive $ by assumption
+  . exact validate_AxiomFive_of_euclidean $ by assumption
+
+end FrameClass.refl_eucl
+
+
 protected abbrev FrameClass.universal : FrameClass := { F | Universal F }
 
-protected abbrev FiniteFrameClass.refl_eucl : FiniteFrameClass := { F | Reflexive F.Rel ∧ Euclidean F.Rel }
+protected abbrev FrameClass.finite_refl_eucl: FrameClass := { F | F.IsFinite ∧ Reflexive F.Rel ∧ Euclidean F.Rel }
 
 lemma iff_validOnUniversalFrameClass_validOnReflexiveEuclideanFrameClass : FrameClass.universal ⊧ φ ↔ Kripke.FrameClass.refl_eucl ⊧ φ := by
   constructor;
@@ -23,27 +42,25 @@ lemma iff_validOnUniversalFrameClass_validOnReflexiveEuclideanFrameClass : Frame
   . rintro h F F_univ;
     exact @h F (⟨refl_of_universal F_univ, eucl_of_universal F_univ⟩);
 
-lemma eq_ReflexiveTransitiveSymmetricFiniteFrameClass_ReflexiveEuclideanFiniteFrameClass : Kripke.FiniteFrameClass.symm_preorder = FiniteFrameClass.refl_eucl := by
+lemma eq_finite_symm_preorder_finite_refl_eucl : Kripke.FrameClass.finite_symm_preorder = FrameClass.finite_refl_eucl := by
   ext F;
   constructor;
-  . rintro ⟨hRefl, hTrans, hSymm⟩;
-    constructor;
+  . rintro ⟨_, hRefl, hTrans, hSymm⟩;
+    refine ⟨inferInstance, ?_, ?_⟩;
     . assumption;
     . exact eucl_of_symm_trans hSymm hTrans;
-  . rintro ⟨hRefl, hEucl⟩;
-    refine ⟨hRefl, ?_, ?_⟩;
+  . rintro ⟨_, hRefl, hEucl⟩;
+    refine ⟨inferInstance, hRefl, ?_, ?_⟩;
     . exact trans_of_refl_eucl hRefl hEucl;
     . exact symm_of_refl_eucl hRefl hEucl;
 
 end Kripke
 
+
 namespace Hilbert.S5.Kripke
 
-instance sound_refl_eucl : Sound (Hilbert.S5) Kripke.FrameClass.refl_eucl := by
-  convert Hilbert.Geach.Kripke.sound (G := {⟨0, 0, 1, 0⟩, ⟨1, 1, 0, 1⟩});
-  exact eq_Geach;
-  . unfold Kripke.FrameClass.refl_eucl FrameClass.multiGeachean MultiGeachean;
-    simp [Geachean.reflexive_def, Geachean.euclidean_def];
+instance sound_refl_eucl : Sound (Hilbert.S5) Kripke.FrameClass.refl_eucl :=
+  instSound_of_validates_axioms Kripke.FrameClass.refl_eucl.validates_HilbertS5
 
 instance sound_universal : Sound (Hilbert.S5) FrameClass.universal := ⟨by
   intro φ hF;
@@ -51,9 +68,8 @@ instance sound_universal : Sound (Hilbert.S5) FrameClass.universal := ⟨by
   exact sound_refl_eucl.sound hF;
 ⟩
 
-instance consistent : Entailment.Consistent (Hilbert.S5) := by
-  convert Hilbert.Geach.Kripke.consistent (G := {⟨0, 0, 1, 0⟩, ⟨1, 1, 0, 1⟩});
-  exact eq_Geach;
+instance consistent : Entailment.Consistent (Hilbert.S5) :=
+  consistent_of_sound_frameclass Kripke.FrameClass.refl_eucl (by simp)
 
 instance canonical : Canonical (Hilbert.S5) Kripke.FrameClass.refl_eucl := ⟨⟨Canonical.reflexive, Canonical.euclidean⟩⟩
 
