Foundation/Modal/Kripke/Undefinability.lean
@@ -4,9 +4,9 @@ namespace LO.Modal
 
 namespace Kripke
 
-abbrev IrreflexiveFrameClass : FrameClass := { F | Irreflexive F }
+abbrev FrameClass.irrefl : FrameClass := { F | Irreflexive F }
 
-theorem undefinable_irreflexive : ¬∃ φ, IrreflexiveFrameClass.DefinedByFormula φ := by
+theorem undefinable_irreflexive : ¬∃ φ, FrameClass.irrefl.DefinedByFormula φ := by
   by_contra hC;
   obtain ⟨φ, ⟨h⟩⟩ := hC;
   replace h : ∀ F : Frame, Irreflexive F ↔ F ⊧ φ := by simpa using h;
