Foundation/Modal/Kripke/Hilbert/K45.lean
@@ -3,21 +3,36 @@ import Foundation.Modal.Kripke.Hilbert.Geach
 namespace LO.Modal
 
 open Kripke
+open Hilbert.Kripke
 open Geachean
 
 protected abbrev Kripke.FrameClass.trans_eucl : FrameClass := { F | Transitive F ∧ Euclidean F }
 
+namespace Kripke.FrameClass.trans_eucl
+
+lemma isMultiGeachean : FrameClass.trans_eucl = FrameClass.multiGeachean {⟨0, 2, 1, 0⟩, ⟨1, 1, 0, 1⟩} := by
+  ext F;
+  simp [Geachean.transitive_def, Geachean.euclidean_def, MultiGeachean]
+
+@[simp]
+lemma nonempty : FrameClass.trans_eucl.Nonempty := by simp [isMultiGeachean]
+
+lemma validates_HilbertK45 : Kripke.FrameClass.trans_eucl.Validates Hilbert.K45.axioms := by
+  apply FrameClass.Validates.withAxiomK;
+  rintro F ⟨F_trans, F_eucl⟩ φ (rfl | rfl);
+  . exact validate_AxiomFour_of_transitive $ by assumption;
+  . exact validate_AxiomFive_of_euclidean $ by assumption;
+
+end Kripke.FrameClass.trans_eucl
+
+
 namespace Hilbert.K45
 
-instance Kripke.sound : Sound (Hilbert.K45) FrameClass.trans_eucl := by
-  convert Hilbert.Geach.Kripke.sound (G := {⟨0, 2, 1, 0⟩, ⟨1, 1, 0, 1⟩});
-  . exact eq_Geach;
-  . unfold FrameClass.trans_eucl FrameClass.multiGeachean MultiGeachean;
-    simp [Geachean.euclidean_def, Geachean.transitive_def];
+instance Kripke.sound : Sound (Hilbert.K45) FrameClass.trans_eucl :=
+  instSound_of_validates_axioms Kripke.FrameClass.trans_eucl.validates_HilbertK45
 
-instance Kripke.consistent : Entailment.Consistent (Hilbert.K45) := by
-  convert Hilbert.Geach.Kripke.consistent (G := {⟨0, 2, 1, 0⟩, ⟨1, 1, 0, 1⟩});
-  exact eq_Geach;
+instance Kripke.consistent : Entailment.Consistent (Hilbert.K45) :=
+  consistent_of_sound_frameclass Kripke.FrameClass.trans_eucl (by simp)
 
 instance Kripke.canonical : Canonical (Hilbert.K45) FrameClass.trans_eucl :=
   ⟨⟨Canonical.transitive, Canonical.euclidean⟩⟩
