Foundation/Modal/Kripke/Hilbert/KD5.lean
@@ -1,27 +1,43 @@
 import Foundation.Modal.Kripke.Hilbert.Geach
-
 namespace LO.Modal
 
 open Kripke
+open Hilbert.Kripke
 open Geachean
 
 abbrev Kripke.FrameClass.serial_eucl : FrameClass := { F | Serial F ∧ Euclidean F }
 
+namespace Kripke.FrameClass.serial_eucl
+
+lemma isMultiGeachean : FrameClass.serial_eucl = FrameClass.multiGeachean {⟨0, 0, 1, 1⟩, ⟨1, 1, 0, 1⟩} := by
+  ext F;
+  simp [Geachean.serial_def, Geachean.euclidean_def, MultiGeachean]
+
+@[simp]
+lemma nonempty : FrameClass.serial_eucl.Nonempty := by simp [isMultiGeachean]
+
+lemma validates_HilbertKD5 : Kripke.FrameClass.serial_eucl.Validates Hilbert.KD5.axioms := by
+  apply FrameClass.Validates.withAxiomK;
+  rintro F ⟨F_serial, F_eucl⟩ φ (rfl | rfl);
+  . exact validate_AxiomD_of_serial $ by assumption;
+  . exact validate_AxiomFive_of_euclidean $ by assumption;
+
+end Kripke.FrameClass.serial_eucl
+
+
+
 namespace Hilbert.KD5
 
-instance Kripke.sound : Sound (Hilbert.KD5) Kripke.FrameClass.serial_eucl := by
-  convert Hilbert.Geach.Kripke.sound (G := {⟨0, 0, 1, 1⟩, ⟨1, 1, 0, 1⟩});
-  . exact eq_Geach;
-  . unfold Kripke.FrameClass.serial_eucl FrameClass.multiGeachean MultiGeachean;
-    simp [Geachean.serial_def, Geachean.euclidean_def];
+instance Kripke.sound : Sound (Hilbert.KD5) Kripke.FrameClass.serial_eucl :=
+  instSound_of_validates_axioms Kripke.FrameClass.serial_eucl.validates_HilbertKD5
 
-instance Kripke.consistent : Entailment.Consistent (Hilbert.KD5) := by
-  convert Hilbert.Geach.Kripke.consistent (G := {⟨0, 0, 1, 1⟩, ⟨1, 1, 0, 1⟩});
-  exact eq_Geach;
+instance Kripke.consistent : Entailment.Consistent (Hilbert.KD5) :=
+  consistent_of_sound_frameclass Kripke.FrameClass.serial_eucl (by simp)
 
 instance Kripke.canonical : Canonical (Hilbert.KD5) Kripke.FrameClass.serial_eucl := ⟨⟨Canonical.serial, Canonical.euclidean⟩⟩
 
 instance Kripke.complete : Complete (Hilbert.KD5) Kripke.FrameClass.serial_eucl := inferInstance
+
 
 end Hilbert.KD5
 
