Foundation/Modal/Kripke/Hilbert/KDB.lean
@@ -3,21 +3,37 @@ import Foundation.Modal.Kripke.Hilbert.Geach
 namespace LO.Modal
 
 open Kripke
+open Hilbert.Kripke
 open Geachean
 
 abbrev Kripke.FrameClass.serial_symm : FrameClass := { F | Serial F ∧ Symmetric F }
 
+namespace Kripke.FrameClass.serial_symm
+
+lemma isMultiGeachean : FrameClass.serial_symm = FrameClass.multiGeachean {⟨0, 0, 1, 1⟩, ⟨0, 1, 0, 1⟩} := by
+  ext F;
+  simp [Geachean.serial_def, Geachean.symmetric_def, MultiGeachean]
+
+@[simp]
+lemma nonempty : FrameClass.serial_symm.Nonempty := by simp [isMultiGeachean]
+
+lemma validates_HilbertKDB : Kripke.FrameClass.serial_symm.Validates Hilbert.KDB.axioms := by
+  apply FrameClass.Validates.withAxiomK;
+  rintro F ⟨F_serial, F_eucl⟩ φ (rfl | rfl);
+  . exact validate_AxiomD_of_serial $ by assumption;
+  . exact validate_AxiomB_of_symmetric $ by assumption;
+
+end Kripke.FrameClass.serial_symm
+
+
+
 namespace Hilbert.KDB
 
-instance Kripke.sound : Sound (Hilbert.KDB) Kripke.FrameClass.serial_symm := by
-  convert Hilbert.Geach.Kripke.sound (G := {⟨0, 0, 1, 1⟩, ⟨0, 1, 0, 1⟩});
-  . exact eq_Geach;
-  . unfold Kripke.FrameClass.serial_symm FrameClass.multiGeachean MultiGeachean;
-    simp [Geachean.serial_def, Geachean.symmetric_def];
+instance Kripke.sound : Sound (Hilbert.KDB) Kripke.FrameClass.serial_symm :=
+  instSound_of_validates_axioms Kripke.FrameClass.serial_symm.validates_HilbertKDB
 
-instance Kripke.consistent : Entailment.Consistent (Hilbert.KDB) := by
-  convert Hilbert.Geach.Kripke.consistent (G := {⟨0, 0, 1, 1⟩, ⟨0, 1, 0, 1⟩});
-  exact eq_Geach;
+instance Kripke.consistent : Entailment.Consistent (Hilbert.KDB) :=
+  consistent_of_sound_frameclass Kripke.FrameClass.serial_symm (by simp)
 
 instance Kripke.canonical : Canonical (Hilbert.KDB) Kripke.FrameClass.serial_symm := ⟨⟨Canonical.serial, Canonical.symmetric⟩⟩
 
