Foundation/Modal/Kripke/Hilbert/S4Point2.lean
@@ -3,21 +3,37 @@ import Foundation.Modal.Kripke.Hilbert.Geach
 namespace LO.Modal
 
 open Kripke
+open Hilbert.Kripke
 open Geachean
 
 abbrev Kripke.FrameClass.confluent_preorder : FrameClass := { F | Reflexive F ∧ Transitive F ∧ Confluent F  }
 
+namespace Kripke.FrameClass.confluent_preorder
+
+lemma isMultiGeachean : FrameClass.confluent_preorder = FrameClass.multiGeachean {⟨0, 0, 1, 0⟩, ⟨0, 2, 1, 0⟩, ⟨1, 1, 1, 1⟩} := by
+  ext F;
+  simp [Geachean.reflexive_def, Geachean.transitive_def, Geachean.confluent_def, MultiGeachean]
+
+@[simp]
+lemma nonempty : FrameClass.confluent_preorder.Nonempty := by simp [isMultiGeachean]
+
+lemma validates_HilbertS4Point2 : Kripke.FrameClass.confluent_preorder.Validates Hilbert.S4Point2.axioms := by
+  apply FrameClass.Validates.withAxiomK;
+  rintro F ⟨F_refl, F_trans, F_conn⟩ φ (rfl | rfl | rfl);
+  . exact validate_AxiomT_of_reflexive F_refl;
+  . exact validate_AxiomFour_of_transitive F_trans;
+  . exact validate_AxiomPoint2_of_confluent F_conn;
+
+end Kripke.FrameClass.confluent_preorder
+
+
 namespace Hilbert.S4Point2
 
-instance Kripke.sound : Sound (Hilbert.S4Point2) Kripke.FrameClass.confluent_preorder := by
-  convert Hilbert.Geach.Kripke.sound (G := {⟨0, 0, 1, 0⟩, ⟨0, 2, 1, 0⟩, ⟨1, 1, 1, 1⟩});
-  . exact eq_Geach;
-  . unfold Kripke.FrameClass.confluent_preorder FrameClass.multiGeachean MultiGeachean;
-    simp [Geachean.reflexive_def, Geachean.transitive_def, Geachean.confluent_def];
+instance Kripke.sound : Sound (Hilbert.S4Point2) Kripke.FrameClass.confluent_preorder :=
+  instSound_of_validates_axioms FrameClass.confluent_preorder.validates_HilbertS4Point2
 
-instance Kripke.consistent : Entailment.Consistent (Hilbert.S4Point2) := by
-  convert Hilbert.Geach.Kripke.consistent (G := {⟨0, 0, 1, 0⟩, ⟨0, 2, 1, 0⟩, ⟨1, 1, 1, 1⟩});
-  exact eq_Geach;
+instance Kripke.consistent : Entailment.Consistent (Hilbert.S4Point2) :=
+  consistent_of_sound_frameclass FrameClass.confluent_preorder (by simp)
 
 instance Kripke.canonical : Canonical (Hilbert.S4Point2) Kripke.FrameClass.confluent_preorder := ⟨⟨Canonical.reflexive, Canonical.transitive, Canonical.confluent⟩⟩
 
