Foundation/Modal/Kripke/Hilbert/Triv.lean
@@ -1,12 +1,32 @@
-import Foundation.Modal.Kripke.Hilbert.Geach
+import Foundation.Modal.Kripke.Hilbert.KT
+import Foundation.Modal.Kripke.Hilbert.KTc
 
 namespace LO.Modal
 
 open Kripke
+open Hilbert.Kripke
 open Geachean
 
 protected abbrev Kripke.FrameClass.refl_corefl : FrameClass := { F | Reflexive F ∧ Coreflexive F }
 protected abbrev Kripke.FrameClass.equality : FrameClass := { F | Equality F }
+
+namespace Kripke.FrameClass.refl_corefl
+
+lemma isMultiGeachean : FrameClass.refl_corefl = FrameClass.multiGeachean {⟨0, 0, 1, 0⟩, ⟨0, 1, 0, 0⟩} := by
+  ext F;
+  simp [Geachean.reflexive_def, Geachean.coreflexive_def, MultiGeachean]
+
+@[simp]
+lemma nonempty : FrameClass.refl_corefl.Nonempty := by simp [isMultiGeachean]
+
+lemma validates_HilbertTriv : Kripke.FrameClass.refl_corefl.Validates Hilbert.Triv.axioms := by
+  apply FrameClass.Validates.withAxiomK;
+  rintro F ⟨F_refl, F_trans⟩ φ (rfl | rfl);
+  . apply FrameClass.refl.validates_AxiomT; repeat tauto;
+  . apply FrameClass.corefl.validates_AxiomTc; repeat tauto;
+
+end Kripke.FrameClass.refl_corefl
+
 
 lemma Kripke.FrameClass.eq_equality_refl_corefl : Kripke.FrameClass.equality = Kripke.FrameClass.refl_corefl := by
   ext F;
@@ -21,19 +41,15 @@ lemma Kripke.FrameClass.eq_equality_refl_corefl : Kripke.FrameClass.equality = K
 
 namespace Hilbert.Triv
 
-instance Kripke.sound_refl_corefl : Sound (Hilbert.Triv) Kripke.FrameClass.refl_corefl := by
-  convert Hilbert.Geach.Kripke.sound (G := {⟨0, 0, 1, 0⟩, ⟨0, 1, 0, 0⟩});
-  exact eq_Geach;
-  . unfold Kripke.FrameClass.refl_corefl FrameClass.multiGeachean MultiGeachean;
-    simp [Geachean.reflexive_def, Geachean.coreflexive_def];
+instance Kripke.sound_refl_corefl : Sound (Hilbert.Triv) Kripke.FrameClass.refl_corefl :=
+  instSound_of_validates_axioms Kripke.FrameClass.refl_corefl.validates_HilbertTriv
 
 instance Kripke.sound_equality : Sound (Hilbert.Triv) Kripke.FrameClass.equality := by
   rw [Kripke.FrameClass.eq_equality_refl_corefl];
   exact Kripke.sound_refl_corefl;
 
-instance Kripke.consistent : Entailment.Consistent (Hilbert.Triv) := by
-  convert Hilbert.Geach.Kripke.consistent (G := {⟨0, 0, 1, 0⟩, ⟨0, 1, 0, 0⟩});
-  exact eq_Geach;
+instance Kripke.consistent : Entailment.Consistent (Hilbert.Triv) :=
+  consistent_of_sound_frameclass Kripke.FrameClass.refl_corefl (by simp)
 
 instance Kripke.cannonical_refl_corefl : Canonical (Hilbert.Triv) Kripke.FrameClass.refl_corefl := ⟨⟨Canonical.reflexive, Canonical.coreflexive⟩⟩
 
